

## Math100B - HW #1

Jay Ser

2026.01.11

**1.**

By the distributive law and cancellation law,  $0r = (0 + 0)r = 0r + 0r \implies 0r = 0$

**2.**

Take any  $a \in \mathbb{Q}$ . Then  $a$  is the root of the linear polynomial  $x - a$ , hence  $a$  is an algebraic number.

**3.**

$(x - (7 + \sqrt{2}))(x - (7 - \sqrt{2})) = (x - 7)^2 - (\sqrt{2})^2 = x^2 - 14x + 47 \in \mathbb{Q}[x]$ . By the above computation,  $7 + \sqrt{2}$  is a root of the polynomial  $x^2 - 14x + 47$ , so it is an algebraic number over  $\mathbb{Q}$ .

Similarly,

$$\begin{aligned} & (x - (\sqrt{3} + \sqrt{-5}))(x - (\sqrt{3} - \sqrt{-5}))(x - (-\sqrt{3} + \sqrt{-5}))(x - (-\sqrt{3} - \sqrt{-5})) \\ &= ((x - \sqrt{3})^2 - (\sqrt{-5})^2)((x + \sqrt{3})^2 - (\sqrt{-5})^2) \\ &= (x^2 - 2\sqrt{3}x + 8)(x^2 + 2\sqrt{3}x + 8) \\ &= x^4 + 16x^2 + 64 - (2\sqrt{3}x)^2 \\ &= x^4 + 4x^2 + 64 \end{aligned}$$

Clearly,  $\sqrt{3} + \sqrt{-5}$  is a root of  $x^4 + 4x^2 + 64 \in \mathbb{Q}[x]$ , so  $\sqrt{3} + \sqrt{-5}$  is an algebraic number over  $\mathbb{Q}$ .

**4.**

Take  $a + b\sqrt{p}, c + d\sqrt{p} \in \mathbb{Z}[\sqrt{p}]$ .

- $(a + b\sqrt{p}) + (c + d\sqrt{p}) = (a + c) + (b + d)\sqrt{p} \in \mathbb{Z}[p]$ .
- $(a + b\sqrt{p})(c + d\sqrt{p}) = (ac + bdp) + (bc + ad)\sqrt{p} \in \mathbb{Z}[p]$ .

Since multiplication and addition are commutative and associative in  $\mathbb{Z}$ , multiplication and addition in  $\mathbb{Z}[\sqrt{p}]$  are commutative and associative too.  $0 + (a + b\sqrt{p}) = a + b\sqrt{p}$  so  $0 \in \mathbb{Z}[\sqrt{p}]$  is the additive identity.  $\forall a + b\sqrt{p} \neq 0 \in \mathbb{Z}[\sqrt{p}]$ ,  $(a + b\sqrt{p}) + (-a + (-b)\sqrt{p}) = 0$ , so every nonzero element has a nonzero identity.  $1 \cdot (a + b\sqrt{p}) = a + b\sqrt{p}$ , so  $1 \in \mathbb{Z}[\sqrt{p}]$  is the multiplicative identity. This verifies that  $\mathbb{Z}[\sqrt{p}]$  is a commutative ring.

Define the following norm function on  $\mathbb{Z}[\sqrt{p}]$ :

$$\lambda : \mathbb{Z}[\sqrt{p}] \rightarrow \mathbb{Z}; \quad a + b\sqrt{p} \rightarrow a^2 - pb^2$$

The following calculation shows that  $\lambda$  is a multiplicative function:

$$\begin{aligned} \lambda(a + b\sqrt{p})\lambda(c + d\sqrt{p}) &= (a^2 - pb^2)(c^2 - pd^2) \\ &= a^2c^2 + p^2b^2d^2 - p(b^2c^2 + a^2d^2) \\ \lambda((a + b\sqrt{p})(c + d\sqrt{p})) &= \lambda(ac + pbd + (bc + ad)\sqrt{p}) \\ &= a^2 + 2pabcd + pb^2d^2 - p(b^2c^2 + 2abcd + a^2d^2) \\ &= a^2c^2 + p^2b^2d^2 - pb^2c^2 - pa^2d^2 \end{aligned}$$

i.e.,  $\lambda(\alpha\beta) = \lambda(\alpha)\lambda(\beta) \forall \alpha, \beta \in \mathbb{Z}[\sqrt{p}]$ .

Suppose  $\alpha \in \mathbb{Z}[\sqrt{p}]$  is a unit. Then  $\exists \beta \in \mathbb{Z}[\sqrt{p}]$  such that  $\alpha\beta = 1$ . Applying the norm on both sides of the equality yields

$$\lambda(\alpha)\lambda(\beta) = 1$$

Since  $\lambda$  maps to the integers,  $\lambda(a) = \pm 1$ .

Conversely, suppose  $\lambda(\alpha) = \pm 1$ . Write  $\alpha = a + b\sqrt{p}$ . Notice that  $\lambda(a + b\sqrt{p}) = (a + b\sqrt{p})(a - b\sqrt{p})$ . So if  $\lambda(\alpha) = 1$ , then  $a - b\sqrt{p}$  is  $\alpha$ 's inverse; if  $\lambda(\alpha) = -1$ , then  $b\sqrt{p} - a$  is  $\alpha$ 's inverse. This shows that  $\alpha \in \mathbb{Z}[\sqrt{p}]$  is a unit  $\iff \lambda(\alpha) = \pm 1$ .

One can define a similar norm function on the Gaussian integers, namely

$$\lambda(a + bi) = a^2 + b^2$$

Notice that  $\lambda$  now maps to only the nonnegative integers with  $\lambda(\alpha) = 0 \iff \alpha = 0$ . Furthermore, the exact same bidirectional proof for the units in  $\mathbb{Z}[i]$  follow:  $a + bi \in \mathbb{Z}[i]$  is a unit  $\iff \lambda(a + bi) = 1$ , where one need not consider the  $\lambda(\alpha) = -1$  anymore.

Specifically,  $\lambda(a + bi) = a^2 + b^2 = 1 \iff a = \pm 1$  and  $b = 0$  or  $a = 0$  and  $b = \pm 1$ . One concludes that the only units of  $\mathbb{Z}[i]$  are  $\pm 1$  and  $\pm i$ .

## 5.

First, here are some trivial calculations.

- $\gamma^3 = 11\sqrt{2} + 9\sqrt{3}$ ,  $\gamma^2 = 5 + 2\sqrt{6}$ .
- The irreducible (minimal) polynomial for  $\gamma$  over  $\mathbb{Z}$ , and thus over  $\mathbb{Q}$ , is  $x^4 - 10x^2 + 1$ .
- Since  $\gamma$  is, well, the sum of  $\sqrt{2}$  and  $\sqrt{3}$ ,  $\gamma \in \mathbb{Q}[\sqrt{2}, \sqrt{3}]$  and  $\gamma \in \mathbb{Z}[\sqrt{2}, \sqrt{3}]$ . Thus  $\mathbb{Z}[\gamma] \subset \mathbb{Z}[\sqrt{2}, \sqrt{3}]$  and  $\mathbb{Q}[\gamma] \subset \mathbb{Q}[\sqrt{2}, \sqrt{3}]$ .

**(a)**  $\mathbb{Q}[\gamma] = \mathbb{Q}[\sqrt{2}, \sqrt{3}]$

It must be shown that  $\sqrt{2}, \sqrt{3} \in \mathbb{Q}[\gamma]$ . Well,  $\gamma^3 = 11\sqrt{2} + 9\sqrt{3}$ , so  $\sqrt{2} = 2^{-1}(\gamma^3 - 9\gamma) \in \mathbb{Q}[\gamma]$  and  $\sqrt{3} = -2^{-1}(\gamma^3 - 11\gamma) \in \mathbb{Q}[\gamma]$ .

**(b)**  $\mathbb{Z}[\gamma] \subsetneq \mathbb{Z}[\sqrt{2}, \sqrt{3}]$

It must be shown that either  $\sqrt{2} \notin \mathbb{Z}[\gamma]$  or  $\sqrt{3} \notin \mathbb{Z}[\gamma]$ . I will cheat and use ring extensions. Since  $x^4 - 10x^2 + 1$  is the irreducible polynomial for  $\gamma$  over  $\mathbb{Z}$ ,

$$\mathbb{Z}[\gamma] \cong \mathbb{Z}[x]/(x^4 - 10x^2 + 1)$$

This is by the First Isomorphism Theorem for rings: consider the substitution homomorphism

$$\varphi : \mathbb{Z}[x] \rightarrow \mathbb{Z}[\gamma]; \quad x \rightarrow \gamma, \quad \varphi|_{\mathbb{Z}} = \text{id}$$

Obviously  $x^4 - 10x^2 + 1 \in \ker \varphi$ , so  $(x^4 - 10x^2 + 1) \subset \ker \varphi$ . Conversely, suppose  $f(x) \in \ker \varphi$ . Dividing  $f(x)$  with remainder by  $x^4 - 10x^2 + 1$ ,

$$f(x) = (x^4 - 10x^2 + 1)q(x) + r(x)$$

where  $r(x) = 0$  or  $\deg r < \deg x^4 - 10x^2 + 1$ . Suppose  $r(x) \neq 0$ . Since  $x^4 - 10x^2 + 1, f(x) \in \ker \varphi$ ,  $r(x) \in \ker \varphi$ . In other words,  $r(\gamma) = 0$  and  $r(x)$  has degree less than  $x^4 - 10x^2 + 1$ . But  $x^4 - 10x^2 + 1$  is the minimal polynomial that has  $\gamma$  as a root, which gives a contradiction. So  $r(x) = 0$ , and  $f(x) \in (x^4 - 10x^2 + 1)$ . This shows that  $\ker \varphi = (x^4 - 10x^2 + 1)$ , and thus  $\mathbb{Z}[x]/(x^4 - 10x^2 + 1) \cong \mathbb{Z}[\gamma]$  by the First Isomorphism Theorem.

Since the irreducible polynomial for  $\gamma$  over  $\mathbb{Z}$  is monic and has degree 4,  $\{1, \gamma, \gamma^2, \gamma^3\}$  form a basis for  $\mathbb{Z}[\gamma]$  over  $\mathbb{Z}$  (view  $\mathbb{Z}[\gamma]$  as  $\mathbb{Z}[x]/(x^4 - 10x^2 + 1)$  and perform division with remainder by  $x^4 - 10x^2 + 1$  in the quotient ring).

Suppose  $\sqrt{2} \in \mathbb{Z}[\gamma]$ . Then  $\exists a_0, \dots, a_3 \in \mathbb{Z}$  such that

$$\sqrt{2} = a_3\gamma^3 + a_2\gamma^2 + a_1\gamma + a_0$$

Substituting the calculated values for  $\gamma^2$  and  $\gamma^3$  yields a system of equations that can easily be solved: On the right hand side,  $\gamma^2$  introduces  $\sqrt{6}$  that is not present in any other term, so  $a_2 = 0$ . Since the left hand side doesn't have any integer part, the sum of integer terms in the left hand side must equal 0. Namely,  $5a_2 + a_0 = 0 \implies a_0 = 0$ . Finally, dealing with the coefficients of  $\sqrt{2}$  and  $\sqrt{3}$  yields the equations  $11a_3 + a_1 = 1$  and  $9a_3 + a_1 = 0$ , which implies  $2a_3 = 1$ . This contradicts the fact that no integer  $a_3$  solves  $2a_3 = 1$ , and thus  $\sqrt{2} \notin \mathbb{Z}[\gamma]$ .

## 6.

$a \in \mathbb{Z}_n$  is a unit  $\iff \exists a' \in \mathbb{Z}_n$  such that  $aa' = 1 \iff \exists a' \in \mathbb{Z}$  such that  $aa' = 1 \pmod n$ . An elementary result from number theory is that the last statement is true if and only if  $(a, n) = 1$ . This shows that the units in  $\mathbb{Z}_n$  are equivalence classes of  $\mathbb{Z}$  that are prime to  $n$ . Since prime numbers are the only integers that are coprime to every number less than it, it follows that  $\mathbb{Z}_n$  is a field if and only if  $n$  is prime.

## 7.

$f(x) := x^2 + x + 1$  is monic, so one can divide  $g(x) := x^4 + 3x^3 + x^2 + 7$  with remainder by  $f(x)$ :

$$x^4 + 3x^3 + x^2 + 7x + 5 = (x^2 + 2x - 2)(x^2 + x + 1) + 7x + 7$$

where  $r(x) := 7x + 7$  is the remainder.

Reducing modulo  $n$ , one sees  $f(x) \mid g(x)$  in  $\mathbb{Z}/n\mathbb{Z} \iff r(x) = 0$  in  $\mathbb{Z}/n\mathbb{Z}$ . Clearly,  $7x + 7 = 0 \pmod n \iff n$  is a multiple of 7, i.e.  $f(x) \mid g(x) \iff 7 \mid n$ .

## 8.

Take  $f(x) = \sum_{i=0}^{\infty} a_i x^i, g(x) = \sum_{i=0}^{\infty} b_i x^i \in F[[t]]$ .

- $f(x) + g(x) = \sum_{i=0}^{\infty} (a_i + b_i) x^i \in F[[t]],$
- $f(x)g(x) = \sum_{i=0}^{\infty} \sum_{j=0}^i a_j x^j b_{i-j} x^{i-j} = \sum_{i=0}^{\infty} \sum_{j=0}^i a_j b_{i-j} x^i \in F[[t]]$

That  $F$  is a field, thus equipped with commutative and associative  $+$  and  $\times$ , allows for an easy verification that addition and multiplication are both commutative and associative in  $F[[t]]$ . As with the polynomial ring, it is easily verified that 0 and 1 are the additive and multiplicative identities of  $F[[t]]$ , respectively. Every  $f(x) \in F[[t]]$  has an additive inverse, namely the polynomial whose coefficient at each index is the additive inverse in  $F$  of the corresponding coefficient in  $f(x)$ . This verifies that  $F[[t]]$  is a commutative ring.

The following shows that  $f(x) = \sum_{i=0}^{\infty} a_i x^i \in F[[t]]$  is a unit  $\iff a_0 \neq 0$ . Suppose  $a_0 = 0$ . Then clearly there is no  $g(x) = \sum_{i=0}^{\infty} b_i x^i$  such that  $f(x)g(x) = 1$  since the constant term is just 0. This shows that if  $f(x)$  is a unit, then  $a_0 \neq 0$ .

Next, take any  $f(x) = \sum_{i=0}^{\infty} a_i x^i \in F[[t]]$  with  $a_i \neq 0$ . Inductively define  $g(x) = \sum_{i=0}^{\infty} b_i x^i \in F[[t]]$ : For  $i = 0$ ,  $b_0 := a_0^{-1}$ . For  $i > 0$ , suppose  $b_0, \dots, b_i$  have been defined. Then let

$$b_{i+1} := a_0^{-1} \left( - \sum_{k=0}^i a_{i-k+1} b_k \right)$$

With this construction, one sees via the definition of multiplication above that  $f(x)g(x) = 1$ : If  $f(x)g(x) = \sum_{i=0}^{\infty} c_i x^i$ , then  $c_0 = a_0 b_0 = 1$ , and for all  $i > 0$ ,

$$b_i = a_0^{-1} \left( - \sum_{k=0}^{i-1} a_{i-k} b_k \right) \implies c_i = \sum_{k=0}^i a_k b_{i-k} = 0$$

\*\* sorry for the messy indexing towards the end, got a rush of sleepiness...